code/Cse230wi25/States.lean
@@ -1,0 +1,13 @@
+set_option pp.fieldNotation false
+set_option pp.proofs true
+
+-- Variables, Values and States -------------------------------
+abbrev Val := Nat
+abbrev Vname := String
+
+abbrev State := Vname -> Val
+-- update state
+def upd (s: State) (x: Vname) (v: Val) : State :=
+  λ y => if y = x then v else s y
+
+notation:10 s " [ " x " := " v " ] " => upd s x v
